
\begin{answer}
	\begin{equation*}
	J(\theta)
	= -\frac{1}{\nexp} \sum_{i=1}^\nexp \left(y^{(i)}\log(h_{\theta}(x^{(i)}))
	+  (1 - y^{(i)})\log(1 - h_{\theta}(x^{(i)}))\right),
	\end{equation*}
	So then
	\begin{align*}
	\nabla J(\theta)
	&= -\frac{1}{n} \sum_{i=1}^n \left(y^{(i)}\frac{1}{h_{\theta}(x^{(i)})} h(1-h) x^{(i)}
	-  (1 - y^{(i)})\frac{1}{1 - h_{\theta}(x^{(i)})} h(1-h) x^{(i)}\right) \\	
	&= -\frac{1}{n} \sum_{i=1}^n \left(x^{(i)} \left[ (1-h) y^{(i)} - (1 - y^{(i)} ) h \right]\right)\\
	&= -\frac{1}{n} \sum_{i=1}^n \left(x^{(i)} \left[ (1-h) y^{(i)} - (1 - y^{(i)} ) h \right]\right)\\
	&= -\frac{1}{n} \sum_{i=1}^n \left(x^{(i)} \left[ y^{(i)} - h \right]\right)\\
	\end{align*}
	And then
	\begin{align*}
	\nabla \nabla J(\theta)
	&= -\frac{1}{n} \sum_{i=1}^n \left( -xx^T h (1-h) \right) = H
	\end{align*}
	So
	\begin{align*}
	z^T H z = \frac{1}{n} \sum_{i=1}^n \left(z x^{(i)} (x^{(i)})^T z^T h_\theta(x^{(i)}) (1 - h_\theta(x^{(i)})) \right) \geq 0
	\end{align*}
	as $h, (1-h) \in (0, 1)$
\end{answer}
