%\input{../macros.tex}
%\begin{document}

\begin{answer}
	\begin{align*}
	p(y = 1\mid x; \phi, \mu_0, \mu_1, \Sigma)
	&= p(x | y=1, \phi, \mu_0, \mu_1, \Sigma) \frac{p(y=1)}{p(x | \phi, \mu_0, \mu_1, \Sigma)} \\
	&= \frac{\phi f_{y=1}(x)}{\phi f_{y=1}(x) + (1-\phi) f_{y=0}(x)}\\
	&= \frac{1}
		{1 + \frac{1-\phi}{\phi} \exp \left(
			 -\frac{1}{2} (x-\mu_1)^T \Sigma^{-1} (x-\mu_1)
			 + \frac{1}{2} (x-\mu_0)^T \Sigma^{-1} (x-\mu_0)
		\right)}\\
	&= \frac{1}{1 + \frac{1-\phi}{\phi} \exp \left(
		- (\mu_0-\mu_1)^T \Sigma^{-1} x 
		- \frac{1}{2}( \mu_1^T \Sigma^{-1} \mu_1 - \mu_0^T \Sigma^{-1} \mu_0)
	\right)}\\ 
	&=\frac{1}{1 + \exp(-(\theta^T x + \theta_0))},
	\end{align*}
\end{answer}

%\end{document}