\input{../macros.tex}
\begin{document}
\begin{answer}
For the semi supervised M-step we maximise over $\theta = \phi, \mu, \Sigma$ while keeping $Q$ fixed the expression $ELBO(Q, \theta) + l_{\text{sup}}(\theta) = \sum_{i=1}^n \sum_{j=1}^k Q_i(z_i)_j \log \frac{p(x_i,z_i; \phi, \mu, \Sigma)}{Q_i(z_i)_j} + \alpha \sum_{i=1}^{\tilde{n}} \log p(x_i, z_i; \phi, \mu, \Sigma)$
\linebreak
So having pre-computed in E-step the fixed $Q_i(z_i)_j = w^i_j$, we can differentiate in turn for each of $\phi, \mu, \Sigma$. Rewriting the whole expression to be maximised as
\begin{equation*}
\sum_{i=1}^n \sum_{j=1}^k w^i_j \log \frac{\phi_j \; N(x_i ; \mu_j, \Sigma_j)}{w^i_j} + \alpha \sum_{i=1}^{\tilde{n}} \log  \left ( \phi_{\tilde{z}_i} \; N(\tilde{x_i} | \tilde{z_i}; \mu, \Sigma) \right )
\end{equation*}
\subsection*{mu}
We get
\begin{align*}
\frac{\partial}{\partial \mu_l} &=
\sum_{i=1}^n w^i_l \frac{\partial}{\partial \mu_l} \log  N(x_i ; \mu_j, \Sigma_j) +
\alpha \sum_{i=1}^{\tilde{n}} \frac{\partial}{\partial \mu_l} \log N(\tilde{x}_i | \tilde{z_i}; \mu, \Sigma)
\\
&= \sum_{i=1}^n w^i_l \Sigma_l^{-1} (x_i - \mu_l) + 
\alpha \sum_{\tilde{z}_i = l} \Sigma_l^{-1} (\tilde{x}_i - \mu_l)
\end{align*}
Setting this to $0$ we get
\begin{align*}
\mu_l =
\frac{
	\sum_{i=1}^n w^i_l x_i + \alpha \sum_{\tilde{z}_i = l} \tilde{x}_i
}
{
	\sum_{i=1}^n w^i_l + \alpha \#\{\tilde{z}_i = l\}
}
\end{align*}
\subsection*{phi}
Similarly for $\phi$ we have
\begin{align*}
\frac{\partial}{\partial \phi_l} = \sum_{i=1}^n w^i_l (1/\phi_l) + \alpha \sum_{\tilde{z}_i = l} (1/\phi_l) = (1/\phi_l) \sum_{i=1}^n w^i_l + \alpha \#\{\tilde{z}_i = l\}
\end{align*}
with constraint that $\sum_l \phi_l = 1$, so we apply the Lagrangian multipliers method:
\begin{align*}
\mathcal{L}(\phi, \lambda) = \sum_{l=1}^k \sum_{i=1}^n w^i_l \log \phi_l + \alpha \#\{\tilde{z}_i = l\} \phi_l \;+\; \lambda( \sum_l \phi_l - 1)
\\
\frac{\partial \mathcal{L}}{\partial \phi_l} = (1/\phi_l) \sum_{i=1}^n w^i_l + \alpha \#\{\tilde{z}_i = l\} \;+\; \lambda = 0
\\
\text{this applies for each $l=1,...,k$, with $\lambda$ constant, so we surmise that}
\\
\phi_l = C \sum_{i=1}^n w^i_l + \alpha \#\{\tilde{z}_i = l\} \quad \text{for some constant $C$, again constant across each $l$}
\\
\text{so applying constraint $\sum_l \phi_l = 1$ we get} \quad
\phi_l = \frac{\sum_{i=1}^n w^i_l + \alpha \#\{\tilde{z}_i = l\}}
{n + \alpha \tilde{n}}
\end{align*}


\subsection*{Sigma}
I cannot be bothered to write this all out again, you get the pattern, so we end up with 
\begin{align*}
\Sigma_l = \frac{\sum_{i=1}^n w^i_l (x_i - \mu_l)(x_i - \mu_l)^T}
{\sum_{i=1}^n w^i_l}
 \;+\;
 \alpha  \frac{\sum_{\tilde{z}_i = l} (\tilde{x}_i - \mu_l)(\tilde{x_i} -  \mu_l)^T}
 {\#{\tilde{z}_i = l}}
\end{align*}
\end{answer}
\end{document}